more

haskell/cfui/Component.hs
@@ -13,18 +13,14 @@ import Console
 
 type Component base w m a = w (UI base m a)
 
-explore :: (Comonad w, Pairing m w) => Component IO w m Console -> IO ()
+explore 
+    :: (Comonad w, Pairing m w) 
+    => Component IO w m Console 
+    -> IO ()
 explore component = do
     ref <- newIORef component
     forever $ do
         space <- readIORef ref
-        let send baction = do
-            action <- baction
-            writeIORef ref (move space action)
-        let Console text action = extract space send
-
-        putStrLn text
-        input <- getLine
-        action input
-
-
+        runConsole $ extract space $ \k -> do
+            act <- k
+            writeIORef ref (move space act)
