haskell/cfui/Components/Counter.hs
@@ -11,20 +11,6 @@ import Console
 import Sequence
 import Component
 
-main :: IO ()
-main = explore counterComponent
-
-_main :: IO ()
-_main = do
-    ref <- newIORef 0
-    forever (ui ref)
-
-ui :: IORef Int -> IO ()
-ui ref = do
-    counter <- readIORef ref 
-    putStrLn (show counter)
-    _ <- getLine
-    writeIORef ref (counter + 1)
 
 counterComponent :: Component IO Stream Sequence Console
 counterComponent = unfoldStream 0 (\state -> (render state, state + 1))
@@ -34,3 +20,20 @@ counterComponent = unfoldStream 0 (\state -> (render state, state + 1))
             Console
                 (show state)                                 
                 (\_input -> send $ return $ (Next (End ()))) 
+
+main :: IO ()
+main = explore counterComponent
+
+_main :: IO ()
+_main = do
+    ref <- newIORef 0
+    forever (_ui ref)
+
+_ui :: IORef Int -> IO ()
+_ui ref = do
+    counter <- readIORef ref 
+    putStrLn (show counter)
+    _ <- getLine
+    writeIORef ref (counter + 1)
+
+
