haskell/cfui/Console.hs
@@ -1,10 +1,17 @@
 module  Console
     (   Console (..)
+    ,   runConsole
     )   where
 
 data Console = Console
-    { _text   :: String
-    , _action :: String -> IO ()
+    { text   :: String
+    , action :: String -> IO ()
     }
+
+runConsole :: Console -> IO ()
+runConsole c = do
+    putStrLn . text $ c
+    input <- getLine
+    action c input
 
 
