haskell/cfui/UI.hs
@@ -2,4 +2,4 @@ module  UI
     (   UI
     )   where
 
-type UI base action a = (base (action ()) -> base ()) -> a
+type UI base m a = (base (m ()) -> base ()) -> a
