coq/Logic/Axiom/Reduction.v
@@ -1,0 +1,18 @@
+Require Import Logic.Axiom.Dec.
+
+Definition red (a b:Type) (p:a -> Prop) (q:b -> Prop) (f:a -> b) : Prop :=
+   forall (x:a), p x <-> q (f x). 
+
+Arguments red {a} {b}.
+
+Lemma redDec : forall (a b:Type) (p:a -> Prop) (q:b -> Prop) (f:a -> b),
+    red p q f -> pDec q -> pDec p.
+Proof.
+    intros a b p q f H1 H2 x. unfold pDec in H2. 
+    unfold red in H1. specialize H1 with x. destruct H1 as [H1 H3].
+    specialize H2 with (f x). destruct H2 as [H2|H2].
+    - left. auto.
+    - right. intros H4. apply H2, H1. assumption.
+Qed.
+
+
